PCDCL: define stgy

Weidenbach_Book/IsaSAT/Pragmatic_CDCL.thy
@@ -345,6 +345,13 @@ inductive pcdcl :: \<open>'v prag_st \<Rightarrow> 'v prag_st \<Rightarrow> bool
   \<open>cdcl_resolution S T \<Longrightarrow> pcdcl S T\<close> |
   \<open>cdcl_subsumed S T \<Longrightarrow> pcdcl S T\<close>
 
+inductive pcdcl_stgy :: \<open>'v prag_st \<Rightarrow> 'v prag_st \<Rightarrow> bool\<close> for S T :: \<open>'v prag_st\<close> where
+  \<open>pcdcl_core_stgy S T \<Longrightarrow> pcdcl_stgy S T\<close> |
+  \<open>cdcl_learn_clause S T \<Longrightarrow> pcdcl_stgy S T\<close> |
+  \<open>cdcl_resolution S T \<Longrightarrow> pcdcl_stgy S T\<close> |
+  \<open>cdcl_subsumed S T \<Longrightarrow> pcdcl_stgy S T\<close>
+
+
 section \<open>Invariants\<close>
 
 text \<open>
@@ -977,7 +984,78 @@ lemma pcdcl_entailed_by_init:
   apply (simp_all add: cdcl_learn_clause_entailed_by_init cdcl_subsumed_entailed_by_init
     cdcl_resolution_entailed_by_init)
   by (meson cdcl\<^sub>W_restart_mset.cdcl\<^sub>W_all_struct_inv_def cdcl\<^sub>W_restart_mset.cdcl\<^sub>W_cdcl\<^sub>W_restart
-  cdcl\<^sub>W_restart_mset.cdcl\<^sub>W_learned_clauses_entailed pcdcl_all_struct_invs_def pcdcl_core_is_cdcl)
+    cdcl\<^sub>W_restart_mset.cdcl\<^sub>W_learned_clauses_entailed pcdcl_all_struct_invs_def pcdcl_core_is_cdcl)
+
+
+
+lemma pcdcl_core_stgy_stgy_invs:
+  assumes
+    confl: \<open>pcdcl_core_stgy S T\<close> and
+    sub: \<open>psubsumed_invs S\<close> and
+    ent: \<open>entailed_clss_inv S\<close> and
+    invs: \<open>cdcl\<^sub>W_restart_mset.cdcl\<^sub>W_all_struct_inv (state\<^sub>W_of S)\<close> and
+     \<open>cdcl\<^sub>W_restart_mset.cdcl\<^sub>W_stgy_invariant (state\<^sub>W_of S)\<close>
+  shows \<open>cdcl\<^sub>W_restart_mset.cdcl\<^sub>W_stgy_invariant (state\<^sub>W_of T)\<close>
+  using assms
+  by (meson cdcl\<^sub>W_restart_mset.cdcl\<^sub>W_stgy_cdcl\<^sub>W_stgy_invariant pcdcl_core_stgy_is_cdcl_stgy)
+
+
+lemma cdcl_subsumed_stgy_stgy_invs:
+  assumes
+    confl: \<open>cdcl_subsumed S T\<close> and
+    sub: \<open>psubsumed_invs S\<close> and
+    ent: \<open>entailed_clss_inv S\<close> and
+    invs: \<open>cdcl\<^sub>W_restart_mset.cdcl\<^sub>W_all_struct_inv (state\<^sub>W_of S)\<close> and
+     \<open>cdcl\<^sub>W_restart_mset.cdcl\<^sub>W_stgy_invariant (state\<^sub>W_of S)\<close>
+  shows \<open>cdcl\<^sub>W_restart_mset.cdcl\<^sub>W_stgy_invariant (state\<^sub>W_of T)\<close>
+  using assms
+  by (induction rule: cdcl_subsumed.induct)
+    (auto simp: cdcl\<^sub>W_restart_mset.cdcl\<^sub>W_stgy_invariant_def
+    cdcl\<^sub>W_restart_mset.no_smaller_confl_def cdcl\<^sub>W_restart_mset.clauses_def)
+
+lemma cdcl_resolution_stgy_stgy_invs:
+  assumes
+    confl: \<open>cdcl_resolution S T\<close> and
+    sub: \<open>psubsumed_invs S\<close> and
+    ent: \<open>entailed_clss_inv S\<close> and
+    invs: \<open>cdcl\<^sub>W_restart_mset.cdcl\<^sub>W_all_struct_inv (state\<^sub>W_of S)\<close> and
+     \<open>cdcl\<^sub>W_restart_mset.cdcl\<^sub>W_stgy_invariant (state\<^sub>W_of S)\<close>
+  shows \<open>cdcl\<^sub>W_restart_mset.cdcl\<^sub>W_stgy_invariant (state\<^sub>W_of T)\<close>
+  using assms
+  by (induction rule: cdcl_resolution.induct)
+    (auto simp: cdcl\<^sub>W_restart_mset.cdcl\<^sub>W_stgy_invariant_def
+    cdcl\<^sub>W_restart_mset.no_smaller_confl_def cdcl\<^sub>W_restart_mset.clauses_def)
+
+
+lemma cdcl_learn_clause_stgy_stgy_invs:
+  assumes
+    confl: \<open>cdcl_learn_clause S T\<close> and
+    sub: \<open>psubsumed_invs S\<close> and
+    ent: \<open>entailed_clss_inv S\<close> and
+    invs: \<open>cdcl\<^sub>W_restart_mset.cdcl\<^sub>W_all_struct_inv (state\<^sub>W_of S)\<close> and
+     \<open>cdcl\<^sub>W_restart_mset.cdcl\<^sub>W_stgy_invariant (state\<^sub>W_of S)\<close>
+  shows \<open>cdcl\<^sub>W_restart_mset.cdcl\<^sub>W_stgy_invariant (state\<^sub>W_of T)\<close>
+  using assms
+  by (induction rule: cdcl_learn_clause.induct)
+    (auto simp: cdcl\<^sub>W_restart_mset.cdcl\<^sub>W_stgy_invariant_def
+    cdcl\<^sub>W_restart_mset.no_smaller_confl_def cdcl\<^sub>W_restart_mset.clauses_def)
+
+
+lemma pcdcl_stgy_stgy_invs:
+  assumes
+    confl: \<open>pcdcl_stgy S T\<close> and
+    sub: \<open>psubsumed_invs S\<close> and
+    ent: \<open>entailed_clss_inv S\<close> and
+    invs: \<open>cdcl\<^sub>W_restart_mset.cdcl\<^sub>W_all_struct_inv (state\<^sub>W_of S)\<close> and
+     \<open>cdcl\<^sub>W_restart_mset.cdcl\<^sub>W_stgy_invariant (state\<^sub>W_of S)\<close>
+  shows \<open>cdcl\<^sub>W_restart_mset.cdcl\<^sub>W_stgy_invariant (state\<^sub>W_of T)\<close>
+  using assms
+  apply (induction rule: pcdcl_stgy.induct)
+  subgoal using pcdcl_core_stgy_stgy_invs by blast
+  subgoal using cdcl_learn_clause_stgy_stgy_invs by blast
+  subgoal using cdcl_resolution_stgy_stgy_invs by blast
+  subgoal using cdcl_subsumed_stgy_stgy_invs by blast
+  done
 
 
 section \<open>Higher-level rules\<close>
